src/Coq_p.hs
@@ -1,0 +1,170 @@
+module Coq_p where
+
+import qualified Prelude
+import qualified Datatypes
+import qualified PeanoNat
+import qualified System.IO
+import Control.Monad
+import qualified Data.Word
+import qualified Data.ByteString as BS
+import System.IO.Error
+
+
+type Handle = System.IO.Handle
+
+type Word8 = Data.Word.Word8
+
+bind :: (Prelude.IO a1) -> (a1 -> Prelude.IO a2) -> Prelude.IO a2
+bind = (>>=)
+
+returnA :: a1 -> Prelude.IO a1
+returnA a =
+  return a
+
+dataSize :: Prelude.Integer
+dataSize = 512
+
+type IOMode = System.IO.IOMode
+
+coq_RO :: IOMode
+coq_RO = System.IO.ReadMode
+
+coq_WO :: IOMode
+coq_WO = System.IO.WriteMode
+
+openFileMy :: Prelude.String -> IOMode -> Prelude.IO
+              (Prelude.Either Prelude.String Handle)
+openFileMy = \x y -> fmap (\e -> case e of 
+              Prelude.Left x -> Prelude.Left (ioeGetErrorString x)
+              Prelude.Right x -> Prelude.Right x) 
+                (System.IO.Error.tryIOError (System.IO.openFile x y))
+
+readFileMy :: Handle -> Prelude.Integer -> Prelude.IO (([]) Word8)
+readFileMy = \x y -> fmap (BS.unpack) (BS.hGet x (Prelude.fromIntegral y))
+
+writeFileMy :: Handle -> (([]) Word8) -> Prelude.IO ()
+writeFileMy = \x y -> BS.hPut x (BS.pack y)
+
+closeFileMy :: Handle -> Prelude.IO ()
+closeFileMy = System.IO.hClose
+
+data Packet =
+   Ack Prelude.Integer
+ | Data Prelude.Integer (([]) Word8)
+ | RRQ Prelude.String
+ | WRQ Prelude.String
+ | Error Prelude.Integer Prelude.String
+ | None
+
+data StateInfo =
+   StateC Handle Prelude.Integer
+
+getNum :: StateInfo -> Prelude.Integer
+getNum a =
+  case a of {
+   StateC _ b -> b}
+
+getFileHandle :: StateInfo -> Handle
+getFileHandle a =
+  case a of {
+   StateC a0 _ -> a0}
+
+data State =
+   Start
+ | WAck StateInfo
+ | WData StateInfo
+ | Exit
+
+incNum :: StateInfo -> StateInfo
+incNum a =
+  case a of {
+   StateC a0 b -> StateC a0 ((Prelude.+) b (Prelude.succ 0))}
+
+nextStep :: State -> Packet -> Prelude.IO ((,) State Packet)
+nextStep s p =
+  case s of {
+   Start ->
+    case p of {
+     RRQ fileName ->
+      bind (openFileMy fileName coq_RO) (\a ->
+        case a of {
+         Prelude.Left s0 -> returnA ((,) Exit (Error (Prelude.succ 0) s0));
+         Prelude.Right f ->
+          bind (readFileMy f dataSize) (\datas ->
+            let {ns = StateC f (Prelude.succ 0)} in
+            case (Prelude.==) (Datatypes.length datas) dataSize of {
+             Prelude.True ->
+              returnA ((,) (WAck ns) (Data (Prelude.succ 0) datas));
+             Prelude.False ->
+              bind (closeFileMy f) (\_ ->
+                returnA ((,) Exit (Data (Prelude.succ 0) datas)))})});
+     WRQ fileName ->
+      bind (openFileMy fileName coq_WO) (\a ->
+        case a of {
+         Prelude.Left s0 -> returnA ((,) Exit (Error (Prelude.succ 0) s0));
+         Prelude.Right f ->
+          returnA ((,) (WData (StateC f (Prelude.succ 0))) (Ack 0))});
+     _ ->
+      returnA ((,) Exit (Error (Prelude.succ (Prelude.succ 0)) ((:) 'U' ((:)
+        'n' ((:) 'r' ((:) 'e' ((:) 'c' ((:) 'o' ((:) 'g' ((:) 'n' ((:) 'i'
+        ((:) 'z' ((:) 'e' ((:) 'd' ((:) ' ' ((:) 'p' ((:) 'a' ((:) 'c' ((:)
+        'k' ((:) 'e' ((:) 't' ((:) ' ' ((:) 't' ((:) 'y' ((:) 'p' ((:) 'e'
+        ([])))))))))))))))))))))))))))};
+   WAck s0 ->
+    case p of {
+     Ack n ->
+      case PeanoNat._Nat__ltb (getNum s0) n of {
+       Prelude.True ->
+        returnA ((,) Exit (Error (Prelude.succ (Prelude.succ (Prelude.succ
+          0))) ((:) 'I' ((:) 'n' ((:) 'c' ((:) 'o' ((:) 'r' ((:) 'r' ((:) 'e'
+          ((:) 'c' ((:) 't' ((:) ' ' ((:) 'p' ((:) 'a' ((:) 'c' ((:) 'k' ((:)
+          'e' ((:) 't' ((:) ' ' ((:) 'n' ((:) 'u' ((:) 'm'
+          ([])))))))))))))))))))))));
+       Prelude.False ->
+        case PeanoNat._Nat__ltb n (getNum s0) of {
+         Prelude.True -> returnA ((,) (WAck s0) None);
+         Prelude.False ->
+          bind (readFileMy (getFileHandle s0) dataSize) (\datas ->
+            let {ns = incNum s0} in
+            case (Prelude.==) (Datatypes.length datas) dataSize of {
+             Prelude.True -> returnA ((,) (WAck ns) (Data (getNum ns) datas));
+             Prelude.False ->
+              bind (closeFileMy (getFileHandle s0)) (\_ ->
+                returnA ((,) Exit (Data (getNum ns) datas)))})}};
+     _ ->
+      bind (closeFileMy (getFileHandle s0)) (\_ ->
+        returnA ((,) Exit (Error (Prelude.succ (Prelude.succ 0)) ((:) 'U'
+          ((:) 'n' ((:) 'r' ((:) 'e' ((:) 'c' ((:) 'o' ((:) 'g' ((:) 'n' ((:)
+          'i' ((:) 'z' ((:) 'e' ((:) 'd' ((:) ' ' ((:) 'p' ((:) 'a' ((:) 'c'
+          ((:) 'k' ((:) 'e' ((:) 't' ((:) ' ' ((:) 't' ((:) 'y' ((:) 'p' ((:)
+          'e' ([]))))))))))))))))))))))))))))};
+   WData s0 ->
+    case p of {
+     Data n datas ->
+      case PeanoNat._Nat__ltb (getNum s0) n of {
+       Prelude.True ->
+        returnA ((,) Exit (Error (Prelude.succ (Prelude.succ (Prelude.succ
+          0))) ((:) 'I' ((:) 'n' ((:) 'c' ((:) 'o' ((:) 'r' ((:) 'r' ((:) 'e'
+          ((:) 'c' ((:) 't' ((:) ' ' ((:) 'p' ((:) 'a' ((:) 'c' ((:) 'k' ((:)
+          'e' ((:) 't' ((:) ' ' ((:) 'n' ((:) 'u' ((:) 'm'
+          ([])))))))))))))))))))))));
+       Prelude.False ->
+        case PeanoNat._Nat__ltb n (getNum s0) of {
+         Prelude.True -> returnA ((,) (WData s0) None);
+         Prelude.False ->
+          bind (writeFileMy (getFileHandle s0) datas) (\_ ->
+            let {ns = incNum s0} in
+            case (Prelude.==) (Datatypes.length datas) dataSize of {
+             Prelude.True -> returnA ((,) (WData ns) (Ack (getNum s0)));
+             Prelude.False ->
+              bind (closeFileMy (getFileHandle s0)) (\_ ->
+                returnA ((,) Exit (Ack (getNum s0))))})}};
+     _ ->
+      bind (closeFileMy (getFileHandle s0)) (\_ ->
+        returnA ((,) Exit (Error (Prelude.succ (Prelude.succ 0)) ((:) 'U'
+          ((:) 'n' ((:) 'r' ((:) 'e' ((:) 'c' ((:) 'o' ((:) 'g' ((:) 'n' ((:)
+          'i' ((:) 'z' ((:) 'e' ((:) 'd' ((:) ' ' ((:) 'p' ((:) 'a' ((:) 'c'
+          ((:) 'k' ((:) 'e' ((:) 't' ((:) ' ' ((:) 't' ((:) 'y' ((:) 'p' ((:)
+          'e' ([]))))))))))))))))))))))))))))};
+   Exit -> returnA ((,) Exit None)}
+
