src/Datatypes.hs
@@ -1,0 +1,10 @@
+module Datatypes where
+
+import qualified Prelude
+
+length :: (([]) a1) -> Prelude.Integer
+length l =
+  case l of {
+   ([]) -> 0;
+   (:) _ l' -> Prelude.succ (length l')}
+
