src/Helpers.hs
@@ -8,25 +8,29 @@ import Data.Maybe
 import System.IO.Error
 import qualified Data.ByteString as BS
 import qualified Data.ByteString.Internal as BS (c2w, w2c)
+import Coq_p
 
-data StateInfo = StateInfo {
-    handle::Handle,
-    number::Int
-} deriving Eq
+instance Eq StateInfo where
+  (StateC f1 f2) == (StateC s1 s2) = f1 == s1 && f2 == s2
+  t1 /= t2 = not (t1 == t2)
 
-data State = Start
-    | WAck StateInfo
-    | WData StateInfo
-    | Exit
-    deriving Eq
-
-data Packet = Ack Int
-    | Data Int BS.ByteString
-    | RRQ String
-    | WRQ String
-    | Error Int String
-    | None
-    deriving Eq
+instance Eq State where
+  (/=) f s = not (f == s)
+  Exit == Exit = True
+  Start == Start = True
+  WAck f1 == WAck s1 = f1 == s1
+  WData f1 == WData f2 = f1 == f2
+  _ == _ = False
+  
+instance Eq Packet where
+  (/=) f s = not (s == f)
+  None == None = True
+  (Ack i1) == (Ack i2) = i1 == i2
+  (Data i1 l1) == (Data i2 l2) = i1 == i2 && l1 == l2
+  (RRQ f1) == (RRQ f2) = f1 == f2
+  (WRQ f1) == (WRQ f2) = f1 == f2
+  (Error i1 e1) == (Error i2 e2) = i1 == i2 && e1 == e2
+  _ == _ = False
 
 getStateInfo::State->Maybe StateInfo
 getStateInfo (WAck s) = Just s
@@ -38,10 +42,10 @@ intToBytes i = [i `div` 256 `mod` 256, i `mod` 256]
 intToBs i = BS.pack $ map fromIntegral $ intToBytes i
 
 convertToBs::Packet -> BS.ByteString
-convertToBs (Ack i) = BS.pack $ map fromIntegral (0:4:(intToBytes i))
-convertToBs (Data i bs) = BS.append (BS.pack [0,3]) $ BS.append (intToBs i) bs
+convertToBs (Ack i) = BS.pack $ map fromIntegral (0:4:(intToBytes (fromIntegral i)))
+convertToBs (Data i bs) = BS.append (BS.pack [0,3]) $ BS.append (intToBs (fromIntegral i)) (BS.pack bs)
 convertToBs (Error i str) = flip BS.append (BS.singleton 0) $ 
-    BS.append (BS.pack [0,5]) $ BS.append (intToBs i) $ BS.pack $ map BS.c2w str
+    BS.append (BS.pack [0,5]) $ BS.append (intToBs (fromIntegral i)) $ BS.pack $ map BS.c2w str
 convertToBs None = BS.empty
 
 convertFromBs::BS.ByteString -> Packet
@@ -51,7 +55,7 @@ convertFromBs bs = let (s,r) = fromJust $ BS.uncons $ BS.tail bs in
             where fileName = map BS.w2c $ takeWhile (/= 0) $ BS.unpack r
         2 -> WRQ fileName
             where fileName = map BS.w2c $ takeWhile (/= 0) $ BS.unpack r
-        3 -> Data num (BS.pack dat)
+        3 -> Data num dat
             where num = (fromIntegral f) * 256 + (fromIntegral s)
                   (f:s:dat) = BS.unpack r
         4 -> Ack num
@@ -62,7 +66,3 @@ convertFromBs bs = let (s,r) = fromJust $ BS.uncons $ BS.tail bs in
                   msg = map BS.w2c $ takeWhile (/= 0) rest
                   (f:s:rest) = BS.unpack r
         _ -> None
-
-incCounter::StateInfo-> StateInfo
-incCounter stateInfo = 
-    StateInfo (handle stateInfo) (number stateInfo + 1)
