Coq_p.v
@@ -1,27 +1,51 @@
 Require Import Coq.Arith.PeanoNat.
+Require Import PeanoNat.
+Require Import Coq.NArith.BinNat.
+Include Coq.Init.Nat.
+Require Import NAxioms NProperties OrdersFacts.
 Require Import Ascii.
 Require Import Coq.Vectors.Vector.
 Require Import Coq.Strings.String.
 Require Import Coq.Lists.List.
 
+Definition Handle := nat.
+
+Definition Word8 := nat.
+
 Inductive Either : Set :=
 | Left: string -> Either
-| Right: nat -> Either.
+| Right: Handle -> Either.
 
+Inductive IO (A:Type) := IOc (a : A).
+
+Definition bind {A B : Type} (a : IO A) (f : A -> IO B) : IO B :=
+  match a with
+  | IOc _ a => f a
+  end.
+
+Definition returnA {A : Type} (a : A) : IO A :=
+  IOc A a.
+
+Axiom dataSize : nat.
+
+Definition IOMode := nat.
+Axiom RO : IOMode.
+Axiom WO : IOMode.
 (*filename->tryb*)
-Axiom openFile:string-> nat -> Either.
-Axiom readFile:nat->nat->list nat.
-Axiom writeFile:nat->list nat-> unit.
-Axiom closeFile:nat->unit.
-Lemma noLongerRead: forall x y : nat, length (readFile x y) <= y.
+Axiom openFileMy:string-> IOMode -> IO Either.
+Axiom readFileMy:Handle->nat-> IO (list Word8).
+Axiom writeFileMy:Handle->list Word8-> IO (unit).
+Axiom closeFileMy:Handle-> IO(unit).
+
+
+Lemma read_less_than_arg :
+  forall (h : Handle) (l : nat), match (readFileMy h l) with | IOc _ a => length a <= l end.
 Proof.
 Admitted.
 
-
-
 Inductive Packet : Set :=
 | Ack : nat -> Packet
-| Data : nat -> list nat -> Packet
+| Data : nat -> list Word8 -> Packet
 | RRQ : string -> Packet
 | WRQ : string -> Packet
 | Error : nat -> string -> Packet
@@ -29,7 +53,7 @@ Inductive Packet : Set :=
 
 (*fileHandle->number*)
 Inductive StateInfo : Type := 
-StateC : nat -> nat -> StateInfo.
+StateC : Handle -> nat -> StateInfo.
 
 Definition getNum (a: StateInfo) :=
   match a with
@@ -62,33 +86,281 @@ Qed.
 
 
 
-Definition nextStep (s : State) (p : Packet) :=
+Definition nextStep (s : State) (p : Packet) : IO (State * Packet) :=
   match s,p with
-  | Start, RRQ fileName => match (openFile fileName 1) with
-                               | Right f => ((WData (StateC f 0)), (Ack 0))
-                               | Left s => (Exit, Error 1 s)
-                               end
-  | Start, WRQ fileName => match (openFile fileName 2) with
-                               | Right f => (WData (StateC f 0), Ack 0)
-                               | Left s => (Exit, Error 1 s)
-                               end
-  | WAck s, Ack n => if ((getNum s) <? n) then (Exit, Error 3 "Incorrect packet num")
-                     else if (n <? getNum s) then (WAck s, None)
-                     else let datas := readFile (getFileHandle s) 512 in
+  | Start, RRQ fileName => bind (openFileMy fileName RO) (fun a => match a with
+                               | Right f => bind (readFileMy f dataSize) ( fun datas =>
+                                    let ns := StateC f 1 in
+                                    if(length datas =? dataSize) then returnA (WAck ns, Data 1 datas)
+                                    else bind (closeFileMy f) ( fun _ =>
+                                        returnA (Exit, Data 1 datas)))
+                               | Left s => returnA (Exit, Error 1 s)
+                               end)
+  | Start, WRQ fileName => bind (openFileMy fileName WO) (fun a => match a with
+                               | Right f => returnA (WData (StateC f 1), Ack 0)
+                               | Left s => returnA (Exit, Error 1 s)
+                               end)
+  | WAck s, Ack n => if ((getNum s) <? n) then returnA (Exit, Error 3 "Incorrect packet num")
+                     else if (n <? getNum s) then returnA (WAck s, None)
+                     else bind (readFileMy (getFileHandle s) dataSize) ( fun datas =>
                           let ns := incNum s in
-                          if(length datas =? 512) then (WAck ns, Data (getNum ns) datas)
-                          else let _ := closeFile (getFileHandle s) in
-                                (Exit, Data (getNum ns) datas)
-  | WData s, Data n datas => if ((getNum s) <? n) then (Exit, Error 3 "Incorrect packet num")
-                             else if (n <? getNum s) then (WData s, None)
-                             else let _ := writeFile (getFileHandle s) datas in
+                          if(length datas =? dataSize) then returnA (WAck ns, Data (getNum ns) datas)
+                          else bind (closeFileMy (getFileHandle s)) ( fun _ =>
+                                returnA (Exit, Data (getNum ns) datas)))
+  | WData s, Data n datas => if ((getNum s) <? n) then returnA (Exit, Error 3 "Incorrect packet num")
+                             else if (n <? getNum s) then returnA (WData s, None)
+                             else bind (writeFileMy (getFileHandle s) datas) (fun _ =>
                                   let ns := incNum s in
-                                  if(length datas =? 512) then (WData ns, Ack (getNum s))
-                                  else let _ := closeFile (getFileHandle s) in
-                                        (Exit, Ack (getNum s))
-  | Start,_ =>  (Exit, Error 2 "Unrecognized packet type")
-  | WAck s, _ => let _ := closeFile (getFileHandle s) in (Exit, Error 2 "Unrecognized packet type")
-  | WData s, _ =>  let _ := closeFile (getFileHandle s) in (Exit, Error 2 "Unrecognized packet type")
-  | Exit, _ => (Exit, None)  
+                                  if(length datas =? dataSize) then returnA (WData ns, Ack (getNum s))
+                                  else bind (closeFileMy (getFileHandle s)) ( fun _ => returnA
+                                        (Exit, Ack (getNum s))))
+  | Start,_ => returnA (Exit, Error 2 "Unrecognized packet type")
+  | WAck s, _ =>bind (closeFileMy (getFileHandle s)) (
+ fun x => returnA (Exit, Error 2 "Unrecognized packet type"))
+  | WData s, _ =>  bind (closeFileMy (getFileHandle s)) (fun _ => returnA (Exit, Error 2 "Unrecognized packet type"))
+  | Exit, _ => returnA (Exit, None)  
   end.
 
+Definition isExitError (a : IO (State * Packet)) : Prop :=
+  match a with
+  | IOc _ (Exit, Error _ _) => True
+  | _ => False
+  end.
+
+Definition isWRQ_RRQ (a: Packet) : Prop :=
+  match a with
+  | WRQ _ => True
+  | RRQ _ => True
+  | _ => False
+  end.
+
+Theorem Start_only_with_RRQ_WRQ : 
+  forall p:Packet, (not (isWRQ_RRQ p)) -> isExitError (nextStep Start p).
+Proof.
+  intros p.
+  unfold not, isWRQ_RRQ, isExitError.
+  simpl.
+  destruct p;unfold returnA; eauto; intros a; destruct a; auto.
+Qed.
+
+Definition is_IO_Left (a : IO Either) :=
+  match a with
+  | IOc _ (Left _) => True
+  | _ => False
+  end.
+
+Definition is_IO_Right (a : IO Either) :=
+  match a with
+  | IOc _ (Right _) => True
+  | _ => False
+  end.
+
+Theorem Exit_on_open_error_RO :
+  forall (fileName : string), 
+    is_IO_Left (openFileMy fileName RO) -> isExitError (nextStep Start (RRQ fileName)).
+Proof.
+  intros fileName.
+  unfold is_IO_Left, nextStep, isExitError, returnA, bind.
+  destruct (openFileMy fileName RO).
+  destruct a; eauto; intros f; inversion f.
+Qed.
+
+Theorem Exit_on_open_error_WO :
+  forall (fileName : string), 
+    is_IO_Left (openFileMy fileName WO) -> isExitError (nextStep Start (WRQ fileName)).
+Proof.
+  intros fileName.
+  unfold is_IO_Left, nextStep, isExitError, returnA, bind.
+  destruct (openFileMy fileName WO).
+  destruct a; eauto; intros f; inversion f.
+Qed.
+
+Definition is_Exit_On_Read_Less_Than_512B (a : IO (State * Packet)) :=
+  match a with
+  | IOc _ (Exit, Data _ d) => length d < dataSize
+  | _ => True
+  end.
+
+Lemma not_le_self : forall (n : nat), n <? n = false.
+Proof.
+  intros n.
+  induction n.
+  auto.
+  auto.
+Qed.
+
+Lemma le_lt_or_eq : forall (n m :nat), n <= m -> n < m \/ n = m.
+Proof.
+  intros n m.
+  intros H.
+  destruct H; try auto.
+  pose proof (Lt.le_lt_n_Sm n m) as p.
+  auto.
+Qed.
+
+Lemma le_if_leq_and_neq : forall (n : nat) (m : nat), n <= m /\ n <> m -> n < m.
+Proof.
+  intros.
+  pose proof (le_lt_or_eq n m) as p.
+  intuition.
+Qed.
+
+Lemma eqn : forall (a: nat) (b : nat), (a =? b) = false <-> a <> b.
+Proof.
+  intros a b.
+  pose proof (Nat.eqb_eq a b) as p.
+  destruct p.
+  remember (a =? b) as eq.
+  destruct eq; intuition.
+Qed.
+
+Theorem Exit_on_read_Less_Than_512B :
+  forall (n : nat) (handle : Handle),
+    is_Exit_On_Read_Less_Than_512B (nextStep (WAck (StateC handle n)) (Ack n)).
+Proof.
+  intros n handle.
+  pose proof (not_le_self n) as pp.
+  unfold is_Exit_On_Read_Less_Than_512B, nextStep, returnA, bind.
+  simpl.
+  destruct (n <? n); try  discriminate.
+  pose proof (read_less_than_arg handle dataSize) as a_l_leq_ds.
+  destruct (readFileMy handle dataSize).
+  remember (Datatypes.length a =? dataSize) as a_l_eq_ds.
+  destruct a_l_eq_ds; auto.
+  remember (closeFileMy handle) as cl.
+  destruct cl.
+  remember (Datatypes.length a) as len_a.
+  pose proof (le_if_leq_and_neq len_a dataSize) as ld.
+  cut (len_a <> dataSize).
+  + intros neq_a.
+    apply ld.
+    auto.
+  + pose proof (eqn len_a dataSize) as p.
+    apply p.
+    symmetry.
+    assumption.
+Qed.
+    
+
+Theorem Exit_on_write_Less_Than_512B :
+  forall (n : nat) (handle : Handle) (d : list Word8),
+    length d <= dataSize -> (match (nextStep (WData (StateC handle n)) (Data n d))with 
+      | IOc _ (Exit, Ack n) => length d < dataSize | _ => True end).
+Proof.
+  intros.
+  unfold nextStep, bind, returnA.
+  simpl.
+  destruct (n <? n); auto.
+  destruct (writeFileMy handle d).
+  remember (Datatypes.length d =? dataSize) as a_l_eq_ds.
+  destruct a_l_eq_ds; auto.
+  remember (closeFileMy handle) as cl.
+  destruct cl.
+  remember (Datatypes.length d) as len_a.
+  pose proof (le_if_leq_and_neq len_a dataSize) as ld.
+  cut (len_a <> dataSize).
+  + intros neq_a.
+    apply ld.
+    auto.
+  + pose proof (eqn len_a dataSize) as p.
+    apply p.
+    symmetry.
+    assumption.
+Qed.
+    
+
+Theorem WRQ_reponds_Ack_0 : 
+  forall (fileName : string),
+    is_IO_Right (openFileMy fileName WO) -> (match (nextStep Start (WRQ fileName)) with 
+    | IOc _ (WData _, Ack 0) => True | _ => False end).
+Proof.
+  intros fileName.
+  unfold is_IO_Right, nextStep, bind, returnA.
+  destruct (openFileMy fileName WO).
+  destruct a; auto.
+Qed.
+
+Theorem NextStep_increment_number_WAck :
+  forall (n : nat) (h: Handle),
+  match (nextStep (WAck (StateC h n)) (Ack n)) with 
+    | IOc _ (WAck s, _) => getNum s = (n+1) | _ => True end.
+Proof.
+  intros n h.
+  unfold nextStep, bind, returnA, getNum.
+  simpl.
+  destruct (n <? n); auto.
+  destruct (readFileMy h dataSize).
+  destruct (closeFileMy h).
+  destruct (Datatypes.length a =? dataSize); auto.
+Qed.
+
+Theorem NextStep_increment_number_WData :
+  forall (n : nat) (h: Handle) (d : list Word8),
+  match (nextStep (WData (StateC h n)) (Data n d)) with 
+    | IOc _ (WData s, _) => getNum s = (n+1) | _ => True end.
+Proof.
+  intros n h d.
+  intros.
+  unfold nextStep, bind, returnA, getNum.
+  simpl.
+  destruct (n <? n); auto.
+  destruct (writeFileMy h d).
+  destruct (closeFileMy h).
+  destruct (Datatypes.length d =? dataSize); auto.
+Qed.
+
+Theorem Old_packets_are_ignored_WAck :
+  forall (n nold : nat) (h : Handle),
+  nold < n -> match nextStep (WAck (StateC h n)) (Ack nold) with
+  | IOc _ (WAck (StateC h n), None) => True | _ => False end.
+Proof.
+  intros n nold h.
+  intros.
+  unfold nextStep, bind, returnA, getNum.
+  simpl.
+  pose proof (Nat.ltb_lt n nold) as p.
+  remember (n <? nold) as nn.
+  destruct nn.
+  + destruct p.
+    pose proof (Nat.lt_asymm n nold) as assym.
+    apply assym; try assumption.
+    apply H0.
+    auto.
+  + pose proof (Nat.ltb_lt nold n) as p2.
+    destruct p2.
+    destruct (nold <? n); auto.
+    pose proof (H1 H) as f.
+    discriminate.
+Qed.
+
+Theorem Old_packets_are_ignored_WData :
+  forall (n nold : nat) (h : Handle) (data: list Word8),
+  nold < n -> match nextStep (WData (StateC h n)) (Data nold data) with
+  | IOc _ (WData (StateC h n), None) => True | _ => False end.
+Proof.
+  intros n nold h data.
+  intros.
+  unfold nextStep, bind, returnA, getNum.
+  simpl.
+  pose proof (Nat.ltb_lt n nold) as p.
+  remember (n <? nold) as nn.
+  destruct nn.
+  + destruct p.
+    pose proof (Nat.lt_asymm n nold) as assym.
+    apply assym; try assumption.
+    apply H0.
+    auto.
+  + pose proof (Nat.ltb_lt nold n) as p2.
+    destruct p2.
+    destruct (nold <? n); auto.
+    pose proof (H1 H) as f.
+    discriminate.
+Qed.
+    
+  
+
+
+
+
+  
+  
