extraction.v
@@ -1,4 +1,4 @@
-Require Coq_p.
+Require Import Coq_p.
 Require Coq.Strings.String.
 
 Extraction Language Haskell.
@@ -9,8 +9,41 @@ Require Import ExtrHaskellNatInteger.
 
 Extraction Blacklist String Int List Nat.
 
-Extract Constant Coq_p.openFile => "openFile".
+Extract Constant Coq_p.openFileMy => 
+"\x y -> fmap (\e -> case e of 
+              Prelude.Left x -> Prelude.Left (ioeGetErrorString x)
+              Prelude.Right x -> Prelude.Right x) 
+                (System.IO.Error.tryIOError (System.IO.openFile x y))".
+Extract Constant Coq_p.readFileMy => "\x y -> fmap (BS.unpack) (BS.hGet x (Prelude.fromIntegral y))".
+Extract Constant Coq_p.writeFileMy => "\x y -> BS.hPut x (BS.pack y)".
+Extract Constant Coq_p.closeFileMy => "System.IO.hClose".
+Extract Constant Coq_p.Word8 => "Data.Word.Word8".
+Extract Constant Coq_p.IOMode => "System.IO.IOMode".
+Extract Constant Coq_p.RO => "System.IO.ReadMode".
+Extract Constant Coq_p.WO => "System.IO.WriteMode".
+Extract Constant Coq_p.Handle => "System.IO.Handle".
+Extract Constant Coq_p.dataSize => "512".
 
-Separate Extraction
-         BinNat BinNums BinInt BinPos (* to jest potrzebne do camlcoq *)
-         Coq_p.
+Extract Inductive Either => "(Prelude.Either Prelude.String Handle)" [ "Prelude.Left" "Prelude.Right" ].
+
+Extract Inductive IO => "Prelude.IO" ["return"].
+Extract Constant bind => "(>>=)".
+
+Module ToExport.
+  Definition RO := Coq_p.RO .
+  Definition WO := Coq_p.WO .
+  Definition dataSize := Coq_p.dataSize.
+  Definition openFileMy := Coq_p.openFileMy .
+  Definition readFileMy := Coq_p.readFileMy .
+  Definition writeFileMy := Coq_p.writeFileMy .
+  Definition closeFileMy := Coq_p.closeFileMy .
+  Definition Packet := Coq_p.Packet .
+  Definition StateInfo := Coq_p.StateInfo .
+  Definition getNum := Coq_p.getNum .
+  Definition getFileHandle := Coq_p.getFileHandle .
+  Definition State := Coq_p.State .
+  Definition incNum := Coq_p.incNum .
+  Definition nextStep := Coq_p.nextStep .
+End ToExport.
+
+Separate Extraction ToExport.
