Makefile
@@ -1,0 +1,15 @@
+all: extract 
+	sed -ie '/^import qualified PeanoNat/a import qualified System.IO\nimport Control.Monad\nimport qualified Data.Word\nimport qualified Data.ByteString as BS\nimport System.IO.Error\n' Coq_p.hs
+	rm -f Top.hs
+	mv -f *.hs ./src
+	stack build
+
+extract: extraction.v Coq_p.vo
+	coqtop -batch -load-vernac-source $<
+
+%.vo: %.v
+	coqc $<
+		
+clean:
+	rm -f *.o *.cmi *.cmo *.cmx *.vo *.hi *.hsi *.hs *.glob *.hse .Coq_p.vo.aux
+	
